coq/Fresh.v
@@ -1,8 +1,10 @@
 Set Implicit Arguments.
+Require Import Strings.String.
 
 Record fresh_state := { counter : nat }.
 
 Definition empty_fresh := {| counter := 0 |}.
 Definition fresh (x : fresh_state) : nat := x.(counter).
+Definition freshv (x : fresh_state) : string := "x"%string.
 Definition advance (x : fresh_state) : fresh_state := {| counter := x.(counter) + 1 |}.
 
